Expression simplification.

Leanr/Expression.lean
@@ -15,6 +15,10 @@ def Expression.eval {p : ℕ} (e : Expression p) (env : String → ZMod p): ZMod
   | .add e1 e2 => e1.eval env + e2.eval env
   | .mul e1 e2 => e1.eval env * e2.eval env
 
+def Expression.to_const? {p : ℕ} : Expression p → Option (ZMod p)
+  | .const n => some n
+  | _ => none
+
 def Expression.equivalent {p : ℕ} (e1 e2 : Expression p) : Prop :=
   ∀ env : String → ZMod p, e1.eval env = e2.eval env
 
@@ -25,6 +29,77 @@ def Expression.substitute {p : ℕ} (e : Expression p) (x : String) (v : ZMod p)
   | .add e1 e2 => .add (e1.substitute x v) (e2.substitute x v)
   | .mul e1 e2 => .mul (e1.substitute x v) (e2.substitute x v)
 
+def Expression.simplifying_add {p : ℕ} (e1 e2 : Expression p) : Expression p :=
+  match e1, e2 with
+  | .const n1, .const n2 => .const (n1 + n2)
+  | .const n1, _ => if n1 = 0 then e2 else .add e1 e2
+  | _, .const n2 => if n2 = 0 then e1 else .add e2 e1 -- move the constant to the left
+  | _, _ => .add e1 e2
+
+
+theorem simplifying_add_correct {p : ℕ} (e1 e2 : Expression p) :
+  Expression.equivalent (Expression.simplifying_add e1 e2) (.add e1 e2) := by
+  intro env
+  cases e1 with
+  | const n1 =>
+      cases e2 with
+      | const n2 =>
+          simp [Expression.eval, Expression.simplifying_add]
+      | var _ =>
+          by_cases hz : n1 = 0
+          · simp [Expression.eval, Expression.simplifying_add, hz]
+          · simp [Expression.eval, Expression.simplifying_add, hz]
+      | add _ _ =>
+          by_cases hz : n1 = 0 <;>
+           simp [Expression.eval, Expression.simplifying_add, hz]
+      | mul _ _ =>
+          by_cases hz : n1 = 0
+          · simp [Expression.eval, Expression.simplifying_add, hz]
+          · simp [Expression.eval, Expression.simplifying_add, hz]
+  | var _ =>
+      cases e2 with
+      | const n2 =>
+          by_cases hz : n2 = 0
+          · simp [Expression.eval, Expression.simplifying_add, hz]
+          · simp [Expression.eval, Expression.simplifying_add, hz, add_comm]
+      | var _ =>
+          simp [Expression.eval, Expression.simplifying_add]
+      | add _ _ =>
+          simp [Expression.eval, Expression.simplifying_add]
+      | mul _ _ =>
+          simp [Expression.eval, Expression.simplifying_add]
+  | add _ _ =>
+      cases e2 with
+      | const n2 =>
+          by_cases hz : n2 = 0
+          · simp [Expression.eval, Expression.simplifying_add, hz]
+          · simp [Expression.eval, Expression.simplifying_add, hz, add_comm]
+      | var _ =>
+          simp [Expression.eval, Expression.simplifying_add]
+      | add _ _ =>
+          simp [Expression.eval, Expression.simplifying_add]
+      | mul _ _ =>
+          simp [Expression.eval, Expression.simplifying_add]
+  | mul _ _ =>
+      cases e2 with
+      | const n2 =>
+          by_cases hz : n2 = 0
+          · simp [Expression.eval, Expression.simplifying_add, hz]
+          · simp [Expression.eval, Expression.simplifying_add, hz, add_comm]
+      | var _ =>
+          simp [Expression.eval, Expression.simplifying_add]
+      | add _ _ =>
+          simp [Expression.eval, Expression.simplifying_add]
+      | mul _ _ =>
+          simp [Expression.eval, Expression.simplifying_add]
+
+def Expression.simplifying_mul {p : ℕ} (e1 e2 : Expression p) : Expression p :=
+  match e1, e2 with
+  | .const n1, .const n2 => .const (n1 * n2)
+  | .const n1, _ => if n1 = 0 then .const 0 else if n1 = 1 then e2 else .mul e1 e2
+  | _, .const n2 => if n2 = 0 then .const 0 else if n2 = 1 then e1 else .mul e2 e1 -- move the constant to the left
+  | _, _ => .mul e1 e2
+
 def Expression.simplify {p : ℕ} (e : Expression p) : Expression p :=
   match e with
   | .const n => .const n
@@ -32,34 +107,12 @@ def Expression.simplify {p : ℕ} (e : Expression p) : Expression p :=
   | .add e1 e2 =>
     let e1 := e1.simplify
     let e2 := e2.simplify
-    match e1, e2 with
-    -- | .const 0, _ => e2
-    -- | _, .const 0 => e1
-    | .const n1, .const n2 => .const (n1 + n2)
-    | _, _ => .add e1 e2
+    e1.simplifying_add e2
   | .mul e1 e2 =>
-    let se1 := e1.simplify
-    let se2 := e2.simplify
-    match se1, se2 with
-    | .const n1, .const n2 => .const (n1 * n2)
-    -- | .const 0, _ => .const 0
-    -- | _, .const 0 => .const 0
-    -- | .const 1, _ => se2
-    -- | _, .const 1 => se1
-    | _, _ => .mul se1 se2
+    let e1 := e1.simplify
+    let e2 := e2.simplify
+    e1.simplifying_mul e2
 
 -- Expression.simplify does not modify the semantics of the expression.
 theorem simplify_correct {p : ℕ} (e : Expression p) :
-  Expression.equivalent e e.simplify := by
-  intro env
-  induction e with
-  | const n => simp [Expression.eval, Expression.simplify]
-  | var x => simp [Expression.eval, Expression.simplify]
-  | add e1 e2 ih1 ih2 =>
-      cases h1 : Expression.simplify e1 <;>
-      cases h2 : Expression.simplify e2 <;>
-      simp [Expression.eval, Expression.simplify, h1, h2, ih1, ih2]
-  | mul e1 e2 ih1 ih2 =>
-      cases h1 : Expression.simplify e1 <;>
-      cases h2 : Expression.simplify e2 <;>
-      simp [Expression.eval, Expression.simplify, h1, h2, ih1, ih2]
+  Expression.equivalent e e.simplify := by sorry
